update the original smt example, comment rust code

examples/smtlib-example/src/lib.rs
@@ -1,37 +1,41 @@
-#[derive(Debug)]
+//! A small example for something that we might want to analyze, and what kind of analysis that
+//! might be.
+//!
+//! First, a message gets verified, and later it gets applied to the state.
+//! Note that this works slightly different to OpenMLS, where the state of the recent verified
+//! messages is kept in the group stata (which is similar to the [`ProtocolLibrary`] in this example.)
+
+
+/// Describes which error occurred.
+#[derive(Debug, PartialEq)]
 enum Error {
     AuthenticationFailed,
     MessageTooOld,
     NotAcceptingNew,
     NotReadyToApply,
+
+    /// When trying to apply a verified message, that verified message is not valid for the current
+    /// state
     UnexpectedVerifiedMsg,
 }
 
-#[derive(Debug)]
-enum State {
-    Idle,
-    WaitToApply{verification_id: usize},
-}
-
+/// The protocol state
 #[derive(Debug)]
 struct ProtocolLibrary {
-    state: State,
     value: usize,
     last_changed: usize,
-    msg_ctr: usize,
 }
 
 impl Default for ProtocolLibrary {
     fn default() -> Self {
         Self {
-            state: State::Idle,
             value: 0,
             last_changed: 0,
-            msg_ctr: 0,
         }
     }
 }
 
+/// An incoming message before validation
 #[derive(Debug)]
 struct UnverifiedMessage {
     sender: usize,
@@ -40,9 +44,25 @@ struct UnverifiedMessage {
     value: usize,
 }
 
+/// This is a relation needed for verification. Says that a message with given timestamp and value
+/// has been sent by the given sender.
+#[hax_lib::opaque]
+fn send(sender: usize, timestamp: usize, value: usize) -> bool {
+    false
+}
+
 #[hax_lib::attributes]
 impl UnverifiedMessage {
-    // this is a bad mac stub
+    // A stupid stub for something like a MAC.
+    //
+    // Since we don't want to translate the body of this function and just want to have it
+    // abstract, we mark it as opaque. Functions with this annotations should be declared, not
+    // defined.
+    //
+    // This function ensures (with no preconditions!) that send holds if the provided timestamp and
+    // value has been verified to originate from the given sender.
+    //
+    // Note that we don't try to prove this postcondition, because the function is opaque,
     #[hax_lib::ensures(|valid| if valid {send(self.sender, self.timestamp, self.value)} else {true})]
     #[hax_lib::opaque]
     fn authenticate(&self) -> bool {
@@ -51,75 +71,55 @@ impl UnverifiedMessage {
 }
 
 
-#[derive(Debug)]
+/// An incoming message after validation
+#[derive(Debug, PartialEq)]
 struct VerifiedMessage {
     sender: usize,
     timestamp: usize,
     value: usize,
     
-    verification_id: usize,
+    /// This describes what version of the state this has been validated for
+    state_last_changed: usize,
 }
 
+#[hax_lib::attributes]
 impl ProtocolLibrary {
-    fn validate(&mut self, msg: &UnverifiedMessage) -> Result<VerifiedMessage, Error> {
-        if !matches!(self.state, State::Idle) {
-            return Err(Error::NotAcceptingNew);
-        }
-
+    /// Validate an incoming message
+    fn validate(&self, msg: &UnverifiedMessage) -> Result<VerifiedMessage, Error> {
         if !msg.authenticate() {
             return Err(Error::AuthenticationFailed);
         }
 
-        if msg.timestamp < self.last_changed {
+        if msg.timestamp <= self.last_changed {
             return Err(Error::MessageTooOld);
         }
-
-        let verification_id = self.msg_ctr;
-
-        self.msg_ctr += 1;
-        self.state = State::WaitToApply{verification_id};
 
         Ok(VerifiedMessage {
             sender: msg.sender,
             value: msg.value,
             timestamp: msg.timestamp,
-            verification_id,
+            state_last_changed: self.last_changed,
         })
     }
 
+    /// Apply an already verified message. Only checks that the validation is not outdated.
+    #[hax_lib::requires(hax_lib::exists(|(s, um): (ProtocolLibrary, &UnverifiedMessage)| -> bool{ Ok(*msg) == s.validate(um)}))]
     fn apply(&mut self, msg: &VerifiedMessage) -> Result<(), Error> {
-        match self.state {
-            State::Idle => return Err(Error::NotReadyToApply),
-            State::WaitToApply{verification_id} => if verification_id != msg.verification_id {
-                return Err(Error::UnexpectedVerifiedMsg)
-            }
+        if self.last_changed != msg.state_last_changed {
+            return Err(Error::UnexpectedVerifiedMsg)
         }
 
         hax_lib::assert!(send(msg.sender, msg.timestamp, msg.value));
+        hax_lib::assert!(msg.timestamp > self.last_changed);
 
         self.value = msg.value;
         self.last_changed = msg.timestamp;
 
         Ok(())
     }
-
-    fn abort(&mut self) -> Result<(), Error> {
-        if !matches!(self.state, State::WaitToApply{..}) {
-            return Err(Error::NotReadyToApply)
-        }
-
-        self.state = State::Idle;
-
-        Ok(())
-    }
-
 }
 
 
-#[hax_lib::opaque]
-fn send(sender: usize, timestamp: usize, value: usize) -> bool {
-    unreachable!()
-}
 
 #[cfg(test)]
 mod tests {
