examples/bitvec-example/bitvec.smt
@@ -1,0 +1,108 @@
+(set-logic ALL)
+
+
+(define-sort bit () (_ BitVec 1))
+(define-sort i16 () (_ BitVec 16))
+(define-sort u8 () (_ BitVec 8))
+
+(define-sort idx16 () (_ BitVec 4))
+(define-sort idx8 () (_ BitVec 1))
+
+(define-sort PortableVector () (Array idx16 i16))
+(define-sort Output () (Array bit u8))
+
+(define-fun load_u8 ((ns PortableVector) (i idx16)) u8
+  ( (_ extract 7 0) (bvand #x00ff (select ns i))))
+
+(echo "sanity checks...")
+(push)
+ (declare-const pv PortableVector)
+ (assert (not (= (load_u8 pv #x0) #x00)))
+ (echo "want sat")
+ (check-sat)
+(pop)
+
+(push)
+ (declare-const pv PortableVector)
+ (assert (= (select pv #x0) #x0121))
+ (assert (= (load_u8 pv #x0) #x21))
+ (echo "want sat")
+ (check-sat)
+(pop)
+
+(push)
+ (declare-const pv PortableVector)
+ (assert (not (=> 
+    (= (select pv #x0) #x0121)
+    (= (load_u8 pv #x0) #x21))))
+ (echo "want unsat")
+ (check-sat)
+(pop)
+
+(define-fun u8_as_bit ((n u8)) bit ((_ int2bv 1) (bv2nat n)))
+(define-fun idx16_as_idx ((n idx16)) idx8 ((_ int2bv 1) (bv2nat (bvlshr n #x3))))
+
+(define-fun
+  serialize-1
+  ((v PortableVector))
+  Output
+  (let
+    ( (o0 (bvor (bvshl (load_u8 v #x0) #x00)
+                (bvshl (load_u8 v #x1) #x01)
+                (bvshl (load_u8 v #x2) #x02)
+                (bvshl (load_u8 v #x3) #x03)
+                (bvshl (load_u8 v #x4) #x04)
+                (bvshl (load_u8 v #x5) #x05)
+                (bvshl (load_u8 v #x6) #x06)
+                (bvshl (load_u8 v #x7) #x07)))
+      (o1 (bvor (bvshl (load_u8 v #x8) #x00)
+                (bvshl (load_u8 v #x9) #x01)
+                (bvshl (load_u8 v #xa) #x02)
+                (bvshl (load_u8 v #xb) #x03)
+                (bvshl (load_u8 v #xc) #x04)
+                (bvshl (load_u8 v #xd) #x05)
+                (bvshl (load_u8 v #xe) #x06)
+                (bvshl (load_u8 v #xf) #x07))))
+      (store (store ((as const Output) #x00) #b0 o0) #b1 o1)))
+
+(define-fun
+  get-bit-pv
+  ( (pv PortableVector)
+    (i idx16))
+  bit
+  ( (_ int2bv 1) (bv2nat (bvand (select pv i) #x0001) )))
+
+
+(define-fun
+  get-bit-packed
+  ( (o Output)
+    (i idx16))
+  bit
+  (let
+    ( (chunk (select o (idx16_as_idx i)))
+      (imod (bvurem i #x8)))
+    (u8_as_bit (bvlshr chunk (concat #x0 imod)))))
+
+
+(declare-const i idx16)
+(declare-const pv PortableVector)
+(declare-const o Output)
+
+(define-fun i16-is-bitty ((v i16)) Bool
+  (= #x0000 (bvand #xfffe v)))
+
+(define-fun PortableVector-is-bitty ((v PortableVector)) Bool
+  (forall ((i idx16)) (i16-is-bitty (select v i))))
+
+(echo "real check: (want unsat)")
+
+; asking for the opposite to find counterexamples
+(assert (not
+      ; the precondition
+  (=> (and  (PortableVector-is-bitty pv)) ; values need to be bits
+            (= o (serialize-1 pv))        ; put the two in relation wrt the encoding
+      ; the postcondition: get-bit is the same
+      (=  (get-bit-packed o  i)
+          (get-bit-pv     pv i)))))
+
+(check-sat)
