examples/smtlib-example/src/example.smt2
@@ -2,13 +2,16 @@
 
 (declare-datatype ~Panicking
   (par (T)
-    ( (~Cont (~Cont/get T))
-      (~Panic))))
+    ( (~cont (~cont/get T))
+      (~panic)
+      (~assert-failed))))
 
 (declare-datatype ~Mutable
   (par (S R)
     ( (~mut (~mut/self S)
             (~mut/return R )))))
+
+(declare-datatype s/Unit ((sc/Unit)))
 
 (declare-datatype e/Result
   (par (T E)
@@ -22,23 +25,17 @@
     ( ev/Error/NotReadyToApply )
     ( ev/Error/UnexpectedVerifiedMsg )))
 
-(declare-datatype e/State
-  ( ( ev/State/Idle )
-    ( ev/State/WaitToApply (evd/State/WaitToApply Int) )))
-
 (declare-datatype s/ProtocolLibrary
   ( (sc/ProtocolLibrary
-      (sd/ProtocolLibrary/state e/State)
       (sd/ProtocolLibrary/value Int)
-      (sd/ProtocolLibrary/last_changed Int)
-      (sd/ProtocolLibrary/msg_ctr Int))))
+      (sd/ProtocolLibrary/last_changed Int))))
 
 (declare-datatype s/UnverifiedMessage
   ( (sc/UnverifiedMessage
       (sd/UnverifiedMessage/sender Int)
-      (sd/UnverifiedMessage/authenticator Int)
       (sd/UnverifiedMessage/timestamp Int)
-      (sd/UnverifiedMessage/value Int))))
+      (sd/UnverifiedMessage/value Int)
+      (sd/UnverifiedMessage/authenticator Int))))
 
 
 (declare-datatype s/VerifiedMessage
@@ -46,59 +43,162 @@
       (sd/VerifiedMessage/sender Int)
       (sd/VerifiedMessage/timestamp Int)
       (sd/VerifiedMessage/value Int)
-      (sd/VerifiedMessage/verification_id Int))))
+      (sd/VerifiedMessage/state_last_changed Int))))
 
-(define-fun
+(declare-fun send (Int Int Int) Bool)
+
+(declare-fun
   fm/UnverifiedMessage/authenticate
-  ((self s/UnverifiedMessage))
-  Bool
-  (= (sd/UnverifiedMessage/authenticator self)
-     (+ (* 2 (sd/UnverifiedMessage/sender self))
-        (* 3 (sd/UnverifiedMessage/value self))
-        (* 5 (sd/UnverifiedMessage/timestamp self)))))
+  ((s/UnverifiedMessage))
+  Bool)
+
+;(define-fun
+;  fm/UnverifiedMessage/authenticate
+;  ((self s/UnverifiedMessage))
+;  Bool
+;  (= (sd/UnverifiedMessage/authenticator self)
+;     (+ (* 2 (sd/UnverifiedMessage/sender self))
+;        (* 3 (sd/UnverifiedMessage/value self))
+;        (* 5 (sd/UnverifiedMessage/timestamp self)))))
+
 
 (define-fun
   fm/ProtocolLibrary/validate
   ( (self s/ProtocolLibrary)
     (msg s/UnverifiedMessage))
-  (~Panicking (~Mutable s/ProtocolLibrary (e/Result s/VerifiedMessage e/Error)))
+  (~Panicking (e/Result s/VerifiedMessage e/Error))
   (ite
-    (is-ev/State/Idle (sd/ProtocolLibrary/state self))
-    (~Cont (~mut self ((as ev/Result/Err (e/Result s/VerifiedMessage e/Error)) ev/Error/NotAcceptingNew)))
+    (not (fm/UnverifiedMessage/authenticate msg))
+    (~cont ((as ev/Result/Err (e/Result s/VerifiedMessage e/Error)) ev/Error/AuthenticationFailed))
     (ite
-      (not (fm/UnverifiedMessage/authenticate msg))
-      (~Cont (~mut self ((as ev/Result/Err (e/Result s/VerifiedMessage e/Error)) ev/Error/AuthenticationFailed)))
+      (<= (sd/UnverifiedMessage/timestamp msg)
+          (sd/ProtocolLibrary/last_changed self))
+      (~cont ((as ev/Result/Err (e/Result s/VerifiedMessage e/Error)) ev/Error/MessageTooOld))
+      (let
+        ( ( self~
+            (sc/ProtocolLibrary
+              (sd/ProtocolLibrary/value self)
+              (sd/ProtocolLibrary/last_changed self))))
+        (~cont 
+          ((as ev/Result/Ok (e/Result s/VerifiedMessage e/Error))
+            (sc/VerifiedMessage
+              (sd/UnverifiedMessage/sender msg)
+              (sd/UnverifiedMessage/timestamp msg)
+              (sd/UnverifiedMessage/value msg)
+              (sd/ProtocolLibrary/last_changed self))))))))
+
+
+(define-fun
+  fm/ProtocolLibrary/apply
+  ( (self s/ProtocolLibrary)
+    (msg  s/VerifiedMessage))
+  (~Panicking (~Mutable s/ProtocolLibrary (e/Result s/Unit e/Error)))
+  (ite
+    (not (= (sd/ProtocolLibrary/last_changed self) (sd/VerifiedMessage/state_last_changed msg)))
+    (~cont (~mut self ((as ev/Result/Err (e/Result s/Unit e/Error)) ev/Error/UnexpectedVerifiedMsg)))
+    (ite
+      (not (send (sd/VerifiedMessage/sender msg) (sd/VerifiedMessage/timestamp msg) (sd/VerifiedMessage/value msg)))
+      (as ~assert-failed (~Panicking (~Mutable s/ProtocolLibrary (e/Result s/Unit e/Error))))
       (ite
-        (<  (sd/UnverifiedMessage/timestamp msg)
-            (sd/ProtocolLibrary/last_changed self))
-        (~Cont (~mut self ((as ev/Result/Err (e/Result s/VerifiedMessage e/Error)) ev/Error/MessageTooOld)))
+        (<= (sd/VerifiedMessage/timestamp msg) (sd/ProtocolLibrary/last_changed self))
+        (as ~assert-failed (~Panicking (~Mutable s/ProtocolLibrary (e/Result s/Unit e/Error))))
         (let
-          ( ( verification_id 
-              (sd/ProtocolLibrary/msg_ctr self)))
-          (let
-            ( ( self~
-                (sc/ProtocolLibrary
-                  (ev/State/WaitToApply verification_id)
-                  (sd/ProtocolLibrary/value self)
-                  (sd/ProtocolLibrary/last_changed self)
-                  (sd/ProtocolLibrary/msg_ctr self))))
-
-            (~Cont (~mut self~
-              ((as ev/Result/Ok (e/Result s/VerifiedMessage e/Error))
-                (sc/VerifiedMessage
-                  (sd/UnverifiedMessage/sender msg)
-                  (sd/UnverifiedMessage/timestamp msg)
-                  (sd/UnverifiedMessage/value msg)
-                  verification_id))))))))))
+          ( ( self~
+              (sc/ProtocolLibrary
+                (sd/VerifiedMessage/value msg)
+                (sd/VerifiedMessage/timestamp msg))))
+          (~cont (~mut self~ ((as ev/Result/Ok (e/Result s/Unit e/Error)) sc/Unit))))))))
 
 
-(declare-const lib  s/ProtocolLibrary)
-(declare-const lib~ s/ProtocolLibrary)
-(declare-const umsg s/UnverifiedMessage)
-(declare-const vmsg s/VerifiedMessage)
 
-(assert (=  (~Cont (~mut lib~ ((as ev/Result/Ok (e/Result s/VerifiedMessage e/Error)) vmsg)))
-            (fm/ProtocolLibrary/validate lib umsg)))
+;; Precondition of UnverifiedMessage::authenticate
+(define-fun
+  pmf/UnverifiedMessage/authenticate/requires
+  ((msg  s/UnverifiedMessage))
+  Bool 
+  true)
 
-(check-sat)
-(get-model)
+;; Postcondition of UnverifiedMessage::authenticate
+(define-fun
+  pmf/UnverifiedMessage/authenticate/ensures
+  ( (msg  s/UnverifiedMessage)
+    (~return Bool))
+  Bool 
+  (=> ~return
+      (send
+        (sd/UnverifiedMessage/sender msg)
+        (sd/UnverifiedMessage/timestamp msg)
+        (sd/UnverifiedMessage/value msg))))
+
+;; Precondition of ProtocolLibrary::apply
+(define-fun
+  pmf/ProtocolLibrary/apply/requires
+  ( (self s/ProtocolLibrary)
+    (msg  s/VerifiedMessage))
+  Bool 
+  (exists 
+    ( (s  s/ProtocolLibrary)
+      (um s/UnverifiedMessage))
+    (=  (fm/ProtocolLibrary/validate s um)
+        (~cont  ( (as ev/Result/Ok
+                      (e/Result s/VerifiedMessage e/Error))
+                  msg)))))
+
+;; Postcondition of ProtocolLibrary::apply
+(define-fun
+  pmf/ProtocolLibrary/apply/ensures
+  ( (self s/ProtocolLibrary)
+    (msg  s/VerifiedMessage)
+    (~return (~Panicking (~Mutable s/ProtocolLibrary (e/Result s/Unit e/Error)))))
+  Bool 
+  (is-~cont ~return))
+
+;;;
+
+; it's an opaque function without preconditions, so we can just require it holds
+(assert (forall
+  ((arg/msg s/UnverifiedMessage))
+  (pmf/UnverifiedMessage/authenticate/ensures
+    arg/msg
+    (fm/UnverifiedMessage/authenticate arg/msg))))
+
+; check ProtocolLibrary/apply claim
+(push)
+  ; args
+  (declare-const arg/self s/ProtocolLibrary)
+  (declare-const arg/msg  s/VerifiedMessage)
+
+  ; return value
+  (define-fun
+    ret
+    ()
+    (~Panicking (~Mutable s/ProtocolLibrary (e/Result s/Unit e/Error)))
+    (fm/ProtocolLibrary/apply arg/self arg/msg))
+
+  ; debug stuff
+  (declare-const simple-ret (~Panicking (~Mutable s/ProtocolLibrary (e/Result s/Unit e/Error))))
+  ;(declare-const s s/ProtocolLibrary)
+  (declare-const um s/UnverifiedMessage)
+  (assert (= ret simple-ret))
+  (assert (=  (fm/ProtocolLibrary/validate arg/self um)
+              (~cont  ( (as ev/Result/Ok
+                            (e/Result s/VerifiedMessage e/Error))
+                        arg/msg))))
+
+  (assert (not (=>
+    (pmf/ProtocolLibrary/apply/requires arg/self arg/msg)
+    (pmf/ProtocolLibrary/apply/ensures arg/self arg/msg ret))))
+
+  (echo "CHECK ProtocolLibrary::apply")
+  (check-sat)
+  (get-model)
+(pop)
+
+; we checked that this holds for valid inputs, can assume it now
+(assert (forall
+  ( (arg/self s/ProtocolLibrary)
+    (arg/msg  s/VerifiedMessage))
+  (pmf/ProtocolLibrary/apply/ensures
+    arg/self
+    arg/msg
+    (fm/ProtocolLibrary/apply arg/self arg/msg))))
